Transformers can decide to evaluate consequence or alternative
For SCCP it is important that only the consequence (alternative) is
considered in the fixpoint iteration if the condition is known to
evaluate to true (false). The transformer can now indicate its choice to
the forward iteration.

Analysis.v
@@ -1,7 +1,7 @@
 Require Import CSet Le.
 
 Require Import Plus Util AllInRel Map.
-Require Import Val Var Env EnvTy IL Annotation Lattice DecSolve LengthEq MoreList.
+Require Import Val Var Env EnvTy IL Annotation Lattice DecSolve LengthEq MoreList Status AllInRel.
 
 Set Implicit Arguments.
 
@@ -9,7 +9,7 @@ Set Implicit Arguments.
 
 Record Analysis (Dom: Type) := makeAnalysis {
   dom_po :> PartialOrder Dom;
-  analysis_step : stmt -> Dom -> Dom;
+  analysis_step : stmt -> Dom -> status Dom;
   initial_value : stmt -> Dom
 }.
 
@@ -18,11 +18,11 @@ Arguments Analysis Dom.
 Section AnalysisAlgorithm.
   Variable Dom : Type.
   Variable analysis : Analysis Dom.
-  Hypothesis first : Dom -> (Dom -> Dom * bool) -> Dom.
+  Hypothesis first : Dom -> (Dom -> status (Dom * bool)) -> status Dom.
 
   Definition step s (d:Dom) :=
-    let d' := analysis_step analysis s d in
-    (d', if [@poLt_dec _ (dom_po analysis) d' d] then false else true).
+    sdo d' <- analysis_step analysis s d;
+    Success (d', if [@poLt _ (dom_po analysis) d' d] then false else true).
 
   Definition fixpoint (s:stmt) :=
     first (initial_value analysis s) (step s).
@@ -32,10 +32,12 @@ End AnalysisAlgorithm.
 Inductive anni (A:Type) : Type :=
 | anni0 : anni A
 | anni1 (a1:A) : anni A
-| anni2 (a1:A) (a2:A) : anni A.
+| anni2 (a1:A) (a2:A) : anni A
+| anni2opt (a1:option A) (a2:option A) : anni A.
 
 Arguments anni A.
 Arguments anni0 [A].
+
 
 Fixpoint setAnni {A} (a:ann A) (ai:anni A) : ann A :=
   match a, ai with
@@ -115,74 +117,85 @@ Definition forward Dom FunDom
     | _, an => an
   end.
 
-Instance PartialOrder_ann Dom `{PartialOrder Dom}
-: PartialOrder (ann Dom) := {
-  poLt := ann_R poLt;
-  poLt_dec := @ann_lt_dec _ _ poLt poLt_dec;
-  poEq := ann_R poEq;
-  poEq_dec := @ann_lt_dec _ _ poEq poEq_dec
-}.
-
-
 Definition makeForwardAnalysis Dom FunDom (BSL:BoundedSemiLattice Dom)
          (ftransform : stmt -> (list FunDom * Dom) -> (list FunDom * anni Dom))
          (fmkFunDom : params -> ann Dom -> FunDom)
 : Analysis (ann Dom) :=
-makeAnalysis _ (fun s d => snd (forward ftransform fmkFunDom s (nil, d))) (fun s => setAnn s bottom).
+makeAnalysis _ (fun s d => Success (snd (forward ftransform fmkFunDom s (nil, d)))) (fun s => setAnn s bottom).
 
 Definition makeBackwardAnalysis Dom FunDom (BSL:BoundedSemiLattice Dom)
            (btransform : list FunDom -> stmt -> anni Dom -> Dom)
            (bmkFunDom : params -> ann Dom -> FunDom)
 : Analysis (ann Dom) :=
 makeAnalysis _
-             (fun s d => backward btransform bmkFunDom s nil d)
+             (fun s d => Success (backward btransform bmkFunDom s nil d))
              (fun s => setAnn s bottom).
 Module SSA.
 
 Definition forward Dom {BSL:BoundedSemiLattice Dom} FunDom
          (ftransform : stmt -> (list FunDom * Dom) -> (list FunDom * anni Dom))
-         (fmkFunDom : params -> Dom -> FunDom) :=
+         (fmkFunDom : params -> Dom -> FunDom)
+         (fgetDom : FunDom -> Dom) :=
   fix forward
       (st:stmt) (a:list FunDom * Dom) {struct st}
-: list FunDom * Dom :=
+  : status (list FunDom * Dom) :=
   match st, a with
     | stmtExp x e s as st, (AL, d) =>
       match ftransform st (AL, d) with
         | (AL, anni1 a) => forward s (AL, a)
-        | _ => (AL, d)
+        | _ => Error "expression transformer failed"
       end
     | stmtIf x s t as st, (AL, d) =>
       match ftransform st (AL, d) with
-        | (AL, anni2 a1 a2) =>
-          let (AL', a1') := forward s (AL, a1) in
-          let (AL'', a2') := forward t (AL', a2) in
-          (AL'', join a1' a2')
-        | _ => (AL, d)
+        | (AL, anni2opt (Some a1) (Some a2)) =>
+          sdo ALds <- forward s (AL, a1);
+          sdo ALdt <- forward t (fst ALds, a2);
+          Success (fst ALdt, join (snd ALds) (snd ALdt))
+        | (AL, anni2opt None (Some a2)) =>
+          forward t (AL, a2)
+        | (AL, anni2opt (Some a1) None) =>
+          forward s (AL, a1)
+        | _ => Error "condition transformer failed"
       end
     | stmtGoto f Y as st, (AL, d) =>
       match ftransform st (AL, d) with
-        | (AL, anni1 a) => (AL, a)
-        | _ => (AL, d)
+        | (AL, anni1 a) => Success (AL, a)
+        | _ => Error "tailcall transformer failed"
       end
     | stmtReturn x as st, (AL, d) =>
       match ftransform st (AL, d) with
-        | (AL, anni1 a) => (AL, a)
-        | _ => (AL, d)
+        | (AL, anni1 a) => Success (AL, a)
+        | _ => Error "return transformer failed"
       end
     | stmtExtern x f Y s as st, (AL, d) =>
       match ftransform st (AL, d) with
         | (AL, anni1 a) => forward s (AL, a)
-        | _ => (AL, d)
+        | _ => Error "syscall transformer failed"
       end
     | stmtLet Z s t as st, (AL, d) =>
-      match ftransform st (fmkFunDom Z d::AL, d) with
-        | (AL, anni2 a1 a2) =>
-          let (AL', a1') := forward s (fmkFunDom Z d::AL, a1) in
-          let (AL'', a2') := forward t (fmkFunDom Z d::AL', a2) in
-          (AL'', join a1' a2')
-        | _ => (AL, d)
+      match ftransform st (fmkFunDom Z bottom::AL, d) with
+        | (AL', anni2 a1 a2) =>
+          sdo ALdt <- forward t (AL', a2);
+          sdo a1' <- option2status (hd_error (fst ALdt)) "FunDom undefined" ;
+          sdo ALds <- forward s (fst ALdt, fgetDom a1');
+          Success (tl (fst ALdt), join (snd ALds) (snd ALdt))
+        | _ => Error "function binding transformer failed"
       end
   end.
+
+(*
+Lemma forward_FunDom_length Dom {BSL:BoundedSemiLattice Dom} FunDom
+         (ftransform : stmt -> (list FunDom * Dom) -> (list FunDom * anni Dom))
+         (fmkFunDom : params -> Dom -> FunDom)
+         s (AL:list FunDom) (a:Dom) r
+ : forward ftransform fmkFunDom s (AL, a) = Success r
+   -> length AL = length (fst r).
+Proof.
+  general induction s; simpl in H.
+  let_case_eq.
+Qed.
+*)
+
 (*
 Definition forward Dom FunDom
          (ftransform : stmt -> (list FunDom * Dom) -> (list FunDom * Dom))
@@ -206,11 +219,12 @@ Definition forward Dom FunDom
   end.
 *)
 
-Definition makeForwardAnalysis Dom FunDom (BSL:BoundedSemiLattice Dom)
+Definition makeForwardAnalysis Dom FunDom (BSL:BoundedSemiLattice Dom) (PO:PartialOrder FunDom)
          (ftransform : stmt -> (list FunDom * Dom) -> (list FunDom * anni Dom))
          (fmkFunDom : params -> Dom -> FunDom)
-: Analysis Dom :=
-makeAnalysis _ (fun s d => snd (forward ftransform fmkFunDom s (nil, d))) (fun s => bottom).
+         fgetDom
+: Analysis (list FunDom * Dom) :=
+makeAnalysis _ (fun s d => forward ftransform fmkFunDom fgetDom s d) (fun s => (nil, bottom)).
 
 
 (*
